Weidenbach_Book/CDCL_W_Level.thy
@@ -5,7 +5,7 @@ begin
 subsubsection \<open>Level of literals and clauses\<close>
 text \<open>Getting the level of a variable, implies that the list has to be reversed. Here is the funtion
   after reversing.\<close>
-fun get_rev_level :: "('v, nat, 'a) marked_lits \<Rightarrow> nat \<Rightarrow> 'v literal \<Rightarrow> nat" where
+fun get_rev_level :: "('v, nat, 'a) ann_literals \<Rightarrow> nat \<Rightarrow> 'v literal \<Rightarrow> nat" where
 "get_rev_level [] _ _ = 0" |
 "get_rev_level (Marked l level # Ls) n L =
   (if atm_of l = atm_of L then level else get_rev_level Ls level L)" |
@@ -20,30 +20,30 @@ lemma get_rev_level_uminus[simp]: "get_rev_level M n(-L) = get_rev_level M n L"
 lemma atm_of_notin_get_rev_level_eq_0[simp]:
   assumes "atm_of L \<notin> atm_of ` lits_of M"
   shows "get_rev_level M n L = 0"
-  using assms by (induct M arbitrary: n rule: marked_lit_list_induct) auto
+  using assms by (induct M arbitrary: n rule: ann_literal_list_induct) auto
 
 lemma get_rev_level_ge_0_atm_of_in:
   assumes  "get_rev_level M n L > n"
   shows "atm_of L \<in> atm_of ` lits_of M"
-  using assms by (induct M arbitrary: n rule: marked_lit_list_induct) fastforce+
+  using assms by (induct M arbitrary: n rule: ann_literal_list_induct) fastforce+
 
 text \<open>In @{const get_rev_level} (resp. @{const get_level}), the beginning (resp. the end) can be
   skipped if the literal is not in the beginning (resp. the end).\<close>
 lemma get_rev_level_skip[simp]:
   assumes  "atm_of L \<notin> atm_of ` lits_of M"
   shows "get_rev_level (M @ Marked K i # M') n L = get_rev_level (Marked K i # M') i L"
-  using assms by (induct M arbitrary: n i rule: marked_lit_list_induct) auto
+  using assms by (induct M arbitrary: n i rule: ann_literal_list_induct) auto
 
 lemma get_rev_level_notin_end[simp]:
   assumes  "atm_of L \<notin> atm_of ` lits_of M'"
   shows "get_rev_level (M @ M') n L = get_rev_level M n L"
-  using assms by (induct M arbitrary: n rule: marked_lit_list_induct) auto
+  using assms by (induct M arbitrary: n rule: ann_literal_list_induct) auto
 
 text \<open>If the literal is at the beginning, then the end can be skipped\<close>
 lemma get_rev_level_skip_end[simp]:
   assumes  "atm_of L \<in> atm_of ` lits_of M"
   shows "get_rev_level (M @ M') n L = get_rev_level M n L"
-  using assms by (induct arbitrary: n rule: marked_lit_list_induct) auto
+  using assms by (induct arbitrary: n rule: ann_literal_list_induct) auto
 
 lemma get_level_skip_beginning:
   assumes "atm_of L' \<noteq> atm_of (lit_of K)"
@@ -54,7 +54,7 @@ lemma get_level_skip_beginning_not_marked_rev:
   assumes "atm_of L \<notin> atm_of ` lit_of `(set S)"
   and "\<forall>s\<in>set S. \<not>is_marked s"
   shows "get_level (M @ rev S) L = get_level M L"
-  using assms by (induction S rule: marked_lit_list_induct) auto
+  using assms by (induction S rule: ann_literal_list_induct) auto
 
 lemma get_level_skip_beginning_not_marked[simp]:
   assumes "atm_of L \<notin> atm_of ` lit_of `(set S)"
@@ -69,11 +69,11 @@ lemma get_rev_level_skip_beginning_not_marked[simp]:
   using get_level_skip_beginning_not_marked_rev[of L "rev S" M] assms by auto
 
 lemma get_level_skip_in_all_not_marked:
-  fixes M :: "('a, nat, 'b) marked_lit list" and L :: "'a literal"
+  fixes M :: "('a, nat, 'b) ann_literal list" and L :: "'a literal"
   assumes "\<forall>m\<in>set M. \<not> is_marked m"
   and "atm_of L \<in> atm_of ` lit_of ` (set M)"
   shows "get_rev_level M n L = n"
-  using assms by (induction M rule: marked_lit_list_induct) auto
+  using assms by (induction M rule: ann_literal_list_induct) auto
 
 lemma get_level_skip_all_not_marked[simp]:
   fixes M
@@ -84,13 +84,13 @@ proof -
   have M: "M = rev M'"
     unfolding M'_def by auto
   show ?thesis
-    using assms unfolding M by (induction M' rule: marked_lit_list_induct) auto
+    using assms unfolding M by (induction M' rule: ann_literal_list_induct) auto
 qed
 
 abbreviation "MMax M \<equiv> Max (set_mset M)"
 
 text \<open>the @{term "{#0#}"}  is there to ensures that the set is not empty.\<close>
-definition get_maximum_level :: "('a, nat, 'b) marked_lit list \<Rightarrow> 'a literal multiset \<Rightarrow> nat"
+definition get_maximum_level :: "('a, nat, 'b) ann_literal list \<Rightarrow> 'a literal multiset \<Rightarrow> nat"
   where
 "get_maximum_level M D = MMax ({#0#} + image_mset (get_level M) D)"
 
@@ -138,7 +138,7 @@ lemma get_maximum_level_skip_first[simp]:
   shows "get_maximum_level (Propagated L C # M) D = get_maximum_level M D"
   using assms unfolding get_maximum_level_def atms_of_def
     atm_of_in_atm_of_set_iff_in_set_or_uminus_in_set
-  by (smt atm_of_in_atm_of_set_in_uminus get_level_skip_beginning image_iff marked_lit.sel(2)
+  by (smt atm_of_in_atm_of_set_in_uminus get_level_skip_beginning image_iff ann_literal.sel(2)
     multiset.map_cong0)
 
 lemma get_maximum_level_skip_beginning:
@@ -175,10 +175,10 @@ lemma get_maximum_level_skip_un_marked_not_present:
   assumes "\<forall>L\<in>#D. atm_of L \<in> atm_of ` lits_of aa" and
   "\<forall>m\<in>set M. \<not> is_marked m"
   shows " get_maximum_level aa D = get_maximum_level (M @ aa) D"
-  using assms by (induction M rule: marked_lit_list_induct)
+  using assms by (induction M rule: ann_literal_list_induct)
   (auto intro!: get_maximum_level_skip_notin[of D "_ @ aa"] simp add: image_Un)
 
-fun get_maximum_possible_level:: "('b, nat, 'c) marked_lit list \<Rightarrow> nat"   where
+fun get_maximum_possible_level:: "('b, nat, 'c) ann_literal list \<Rightarrow> nat"   where
 "get_maximum_possible_level [] = 0" |
 "get_maximum_possible_level (Marked K i # l) = max i (get_maximum_possible_level l)" |
 "get_maximum_possible_level (Propagated _ _ # l) = get_maximum_possible_level l"
@@ -186,15 +186,15 @@ fun get_maximum_possible_level:: "('b, nat, 'c) marked_lit list \<Rightarrow> na
 lemma get_maximum_possible_level_append[simp]:
   "get_maximum_possible_level (M@M')
     = max (get_maximum_possible_level M) (get_maximum_possible_level M')"
-  by (induct M rule: marked_lit_list_induct) auto
+  by (induct M rule: ann_literal_list_induct) auto
 
 lemma get_maximum_possible_level_rev[simp]:
   "get_maximum_possible_level (rev M) = get_maximum_possible_level M"
-  by (induct M rule: marked_lit_list_induct) auto
+  by (induct M rule: ann_literal_list_induct) auto
 
 lemma get_maximum_possible_level_ge_get_rev_level:
   "max (get_maximum_possible_level M) i \<ge> get_rev_level M i L"
-  by (induct M arbitrary: i rule: marked_lit_list_induct) (auto simp add: le_max_iff_disj)
+  by (induct M arbitrary: i rule: ann_literal_list_induct) (auto simp add: le_max_iff_disj)
 
 lemma get_maximum_possible_level_ge_get_level[simp]:
   "get_maximum_possible_level M \<ge> get_level M L"
@@ -212,17 +212,17 @@ fun get_all_mark_of_propagated where
 
 lemma get_all_mark_of_propagated_append[simp]:
   "get_all_mark_of_propagated (A @ B) = get_all_mark_of_propagated A @ get_all_mark_of_propagated B"
-  by (induct A rule: marked_lit_list_induct) auto
+  by (induct A rule: ann_literal_list_induct) auto
 
 subsubsection \<open>Properties about the levels\<close>
-fun get_all_levels_of_marked :: "('b, 'a, 'c) marked_lit list \<Rightarrow> 'a list"  where
+fun get_all_levels_of_marked :: "('b, 'a, 'c) ann_literal list \<Rightarrow> 'a list"  where
 "get_all_levels_of_marked [] = []" |
 "get_all_levels_of_marked (Marked l level # Ls) = level # get_all_levels_of_marked Ls" |
 "get_all_levels_of_marked (Propagated _ _ # Ls) = get_all_levels_of_marked Ls"
 
 lemma get_all_levels_of_marked_nil_iff_not_is_marked:
   "get_all_levels_of_marked xs = [] \<longleftrightarrow> (\<forall> x \<in> set xs. \<not>is_marked x)"
-  using assms by (induction xs rule: marked_lit_list_induct) auto
+  using assms by (induction xs rule: ann_literal_list_induct) auto
 
 lemma get_all_levels_of_marked_cons:
   "get_all_levels_of_marked (a # b) =
@@ -241,7 +241,7 @@ proof
 next
   assume ?A
   then show ?B
-    apply (induction M rule: marked_lit_list_induct)
+    apply (induction M rule: ann_literal_list_induct)
       apply auto[]
      apply (metis append_Cons append_Nil get_all_levels_of_marked.simps(2) set_ConsD)
     by (metis append_Cons get_all_levels_of_marked.simps(3))
@@ -265,15 +265,15 @@ lemma get_all_levels_of_marked_rev_eq_rev_get_all_levels_of_marked[simp]:
 
 lemma get_maximum_possible_level_max_get_all_levels_of_marked:
   "get_maximum_possible_level M = Max (insert 0 (set (get_all_levels_of_marked M)))"
-  by (induct M rule: marked_lit_list_induct) (auto simp: insert_commute)
+  by (induct M rule: ann_literal_list_induct) (auto simp: insert_commute)
 
 lemma get_rev_level_in_levels_of_marked:
   "get_rev_level M n L \<in> {0, n} \<union> set (get_all_levels_of_marked M)"
-  by (induction M arbitrary: n rule: marked_lit_list_induct) (force simp add: atm_of_eq_atm_of)+
+  by (induction M arbitrary: n rule: ann_literal_list_induct) (force simp add: atm_of_eq_atm_of)+
 
 lemma get_rev_level_in_atms_in_levels_of_marked:
   "atm_of L \<in> atm_of ` (lits_of M) \<Longrightarrow> get_rev_level M n L \<in> {n} \<union> set (get_all_levels_of_marked M)"
-  by (induction M arbitrary: n rule: marked_lit_list_induct) (auto simp add: atm_of_eq_atm_of)
+  by (induction M arbitrary: n rule: ann_literal_list_induct) (auto simp add: atm_of_eq_atm_of)
 
 
 lemma get_all_levels_of_marked_no_marked:
@@ -311,7 +311,7 @@ lemma get_rev_level_can_skip_correctly_ordered:
     "get_all_levels_of_marked M = rev [Suc 0..<Suc (length (get_all_levels_of_marked M))]"
   shows "get_rev_level (rev M @ K) 0 L = get_rev_level K (length (get_all_levels_of_marked M)) L"
   using assms
-proof (induct M arbitrary: K rule: marked_lit_list_induct)
+proof (induct M arbitrary: K rule: ann_literal_list_induct)
   case nil
   then show ?case by simp
 next
@@ -339,7 +339,7 @@ lemma get_level_skip_beginning_hd_get_all_levels_of_marked:
   and "get_all_levels_of_marked S \<noteq> []"
   shows "get_level (M@ S) L = get_rev_level (rev M) (hd (get_all_levels_of_marked S)) L"
   using assms
-proof (induction S arbitrary: M rule: marked_lit_list_induct)
+proof (induction S arbitrary: M rule: ann_literal_list_induct)
   case nil
   then show ?case by (auto simp add: lits_of_def)
 next
