Weidenbach_Book/DPLL_W_Implementation.thy
@@ -4,8 +4,8 @@ begin
 
 subsection \<open>Simple Implementation of DPLL\<close>
 subsubsection \<open>Combining the propagate and decide: a DPLL step\<close>
-definition DPLL_step :: "int dpll\<^sub>W_marked_lits \<times> int literal list list
-  \<Rightarrow> int dpll\<^sub>W_marked_lits \<times> int literal list list"  where
+definition DPLL_step :: "int dpll\<^sub>W_ann_literals \<times> int literal list list
+  \<Rightarrow> int dpll\<^sub>W_ann_literals \<times> int literal list list"  where
 "DPLL_step = (\<lambda>(Ms, N).
   (case find_first_unit_clause N Ms of
     Some (L, _) \<Rightarrow> (Propagated L () # Ms, N)
@@ -26,9 +26,9 @@ value "DPLL_step ([Marked (Neg 1) ()], [[Pos (1::int), Neg 2]])"
 
 text \<open>We define the conversion function between the states as defined in \<open>Prop_DPLL\<close> (with
   multisets) and here (with lists).\<close>
-abbreviation "toS \<equiv> \<lambda>(Ms::(int, unit, unit) marked_lit list)
+abbreviation "toS \<equiv> \<lambda>(Ms::(int, unit, unit) ann_literal list)
                       (N:: int literal list list). (Ms, mset (map mset N)) "
-abbreviation "toS' \<equiv> \<lambda>(Ms::(int, unit, unit) marked_lit list,
+abbreviation "toS' \<equiv> \<lambda>(Ms::(int, unit, unit) ann_literal list,
                           N:: int literal list list). (Ms, mset (map mset N)) "
 
 text \<open>Proof of correctness of @{term DPLL_step}\<close>
@@ -144,8 +144,8 @@ qed
 
 subsubsection \<open>Adding invariants\<close>
 paragraph \<open>Invariant tested in the function\<close>
-function DPLL_ci :: "int dpll\<^sub>W_marked_lits \<Rightarrow> int literal list list
-  \<Rightarrow> int dpll\<^sub>W_marked_lits \<times> int literal list list" where
+function DPLL_ci :: "int dpll\<^sub>W_ann_literals \<Rightarrow> int literal list list
+  \<Rightarrow> int dpll\<^sub>W_ann_literals \<times> int literal list list" where
 "DPLL_ci Ms N =
   (if \<not>dpll\<^sub>W_all_inv (Ms, mset (map mset N))
   then (Ms, N)
@@ -158,7 +158,7 @@ proof (relation "{(S', S).  (toS' S', toS' S) \<in> {(S', S). dpll\<^sub>W_all_i
   show  "wf {(S', S).(toS' S', toS' S) \<in> {(S', S). dpll\<^sub>W_all_inv S \<and> dpll\<^sub>W S S'}}"
     using  wf_if_measure_f[OF dpll\<^sub>W_wf, of "toS'"] by auto
 next
-  fix Ms :: "int dpll\<^sub>W_marked_lits" and N x xa y
+  fix Ms :: "int dpll\<^sub>W_ann_literals" and N x xa y
   assume"\<not> \<not> dpll\<^sub>W_all_inv (toS Ms N)"
   and step: "x = DPLL_step (Ms, N)"
   and x: "(xa, y) = x"
@@ -168,8 +168,8 @@ next
 qed
 
 paragraph \<open>No invariant tested\<close>
-function (domintros) DPLL_part:: "int dpll\<^sub>W_marked_lits \<Rightarrow> int literal list list \<Rightarrow>
-  int dpll\<^sub>W_marked_lits \<times> int literal list list" where
+function (domintros) DPLL_part:: "int dpll\<^sub>W_ann_literals \<Rightarrow> int literal list list \<Rightarrow>
+  int dpll\<^sub>W_ann_literals \<times> int literal list list" where
 "DPLL_part Ms N =
   (let (Ms', N') = DPLL_step (Ms, N) in
    if (Ms', N') = (Ms, N) then (Ms, N) else DPLL_part Ms' N)"
@@ -342,7 +342,7 @@ qed
 
 
 lemma DPLL_part_dpll\<^sub>W_all_inv_final:
-  fixes M Ms':: "(int, unit, unit) marked_lit list" and
+  fixes M Ms':: "(int, unit, unit) ann_literal list" and
     N :: "int literal list list"
   assumes inv: "dpll\<^sub>W_all_inv (Ms, mset (map mset N))"
   and MsN: "DPLL_part Ms N = (Ms', N)"
@@ -357,7 +357,7 @@ qed
 paragraph \<open>Embedding the invariant into the type\<close>
 paragraph \<open>Defining the type\<close>
 typedef dpll\<^sub>W_state =
-    "{(M::(int, unit, unit) marked_lit list, N::int literal list list).
+    "{(M::(int, unit, unit) ann_literal list, N::int literal list list).
         dpll\<^sub>W_all_inv (toS M N)}"
   morphisms rough_state_of state_of
 proof
@@ -517,7 +517,7 @@ qed
 
 subsubsection \<open>Code export\<close>
 paragraph \<open>A conversion to @{typ dpll\<^sub>W_state}\<close>
-definition Con :: "(int, unit, unit) marked_lit list \<times> int literal list list
+definition Con :: "(int, unit, unit) ann_literal list \<times> int literal list list
                      \<Rightarrow> dpll\<^sub>W_state" where
   "Con xs = state_of (if dpll\<^sub>W_all_inv (toS (fst xs) (snd xs)) then xs else ([], []))"
 lemma [code abstype]:
@@ -681,32 +681,32 @@ fun uminus_literal l = (if is_pos l then Neg else Pos) (atm_of l);
 end; (*struct Clausal_Logic*)
 
 structure Partial_Annotated_Clausal_Logic : sig
-  datatype ('a, 'b, 'c) marked_lit = Marked of 'a Clausal_Logic.literal * 'b |
+  datatype ('a, 'b, 'c) ann_literal = Marked of 'a Clausal_Logic.literal * 'b |
     Propagated of 'a Clausal_Logic.literal * 'c
-  val equal_marked_lit :
+  val equal_ann_literal :
     'a HOL.equal -> 'b HOL.equal -> 'c HOL.equal ->
-      ('a, 'b, 'c) marked_lit HOL.equal
-  val lit_of : ('a, 'b, 'c) marked_lit -> 'a Clausal_Logic.literal
-  val lits_of : ('a, 'b, 'c) marked_lit list -> 'a Clausal_Logic.literal Set.set
+      ('a, 'b, 'c) ann_literal HOL.equal
+  val lit_of : ('a, 'b, 'c) ann_literal -> 'a Clausal_Logic.literal
+  val lits_of : ('a, 'b, 'c) ann_literal list -> 'a Clausal_Logic.literal Set.set
   val backtrack_split :
-    ('a, 'b, 'c) marked_lit list ->
-      ('a, 'b, 'c) marked_lit list * ('a, 'b, 'c) marked_lit list
+    ('a, 'b, 'c) ann_literal list ->
+      ('a, 'b, 'c) ann_literal list * ('a, 'b, 'c) ann_literal list
 end = struct
 
-datatype ('a, 'b, 'c) marked_lit = Marked of 'a Clausal_Logic.literal * 'b |
+datatype ('a, 'b, 'c) ann_literal = Marked of 'a Clausal_Logic.literal * 'b |
   Propagated of 'a Clausal_Logic.literal * 'c;
 
-fun equal_marked_lita A_ B_ C_ (Marked (x11, x12)) (Propagated (x21, x22)) =
+fun equal_ann_literala A_ B_ C_ (Marked (x11, x12)) (Propagated (x21, x22)) =
   false
-  | equal_marked_lita A_ B_ C_ (Propagated (x21, x22)) (Marked (x11, x12)) =
+  | equal_ann_literala A_ B_ C_ (Propagated (x21, x22)) (Marked (x11, x12)) =
     false
-  | equal_marked_lita A_ B_ C_ (Propagated (x21, x22)) (Propagated (y21, y22)) =
+  | equal_ann_literala A_ B_ C_ (Propagated (x21, x22)) (Propagated (y21, y22)) =
     Clausal_Logic.equal_literala A_ x21 y21 andalso HOL.eq C_ x22 y22
-  | equal_marked_lita A_ B_ C_ (Marked (x11, x12)) (Marked (y11, y12)) =
+  | equal_ann_literala A_ B_ C_ (Marked (x11, x12)) (Marked (y11, y12)) =
     Clausal_Logic.equal_literala A_ x11 y11 andalso HOL.eq B_ x12 y12;
 
-fun equal_marked_lit A_ B_ C_ = {equal = equal_marked_lita A_ B_ C_} :
-  ('a, 'b, 'c) marked_lit HOL.equal;
+fun equal_ann_literal A_ B_ C_ = {equal = equal_ann_literala A_ B_ C_} :
+  ('a, 'b, 'c) ann_literal HOL.equal;
 
 fun lit_of (Marked (x11, x12)) = x11
   | lit_of (Propagated (x21, x22)) = x21;
@@ -728,7 +728,7 @@ structure DPLL_CDCL_W_Implementation : sig
   val find_first_unit_clause :
     'a HOL.equal ->
       ('a Clausal_Logic.literal list) list ->
-        ('a, 'b, 'c) Partial_Annotated_Clausal_Logic.marked_lit list ->
+        ('a, 'b, 'c) Partial_Annotated_Clausal_Logic.ann_literal list ->
           ('a Clausal_Logic.literal * 'a Clausal_Logic.literal list) option
 end = struct
 
@@ -772,17 +772,17 @@ end; (*struct DPLL_CDCL_W_Implementation*)
 structure DPLL_W_Implementation : sig
   datatype dpll_W_state =
   Con of
-    ((Arith.int, unit, unit) Partial_Annotated_Clausal_Logic.marked_lit list *
+    ((Arith.int, unit, unit) Partial_Annotated_Clausal_Logic.ann_literal list *
       (Arith.int Clausal_Logic.literal list) list);
   val dPLL_tot_rep :
     dpll_W_state ->
       bool *
-        (Arith.int, unit, unit) Partial_Annotated_Clausal_Logic.marked_lit list
+        (Arith.int, unit, unit) Partial_Annotated_Clausal_Logic.ann_literal list
 end = struct
 
 datatype dpll_W_state =
   Con of
-    ((Arith.int, unit, unit) Partial_Annotated_Clausal_Logic.marked_lit list *
+    ((Arith.int, unit, unit) Partial_Annotated_Clausal_Logic.ann_literal list *
       (Arith.int Clausal_Logic.literal list) list);
 
 fun rough_state_of (Con x) = x;
@@ -790,7 +790,7 @@ fun rough_state_of (Con x) = x;
 fun equal_dpll_W_state sa s =
   Product_Type.equal_prod
     (List.equal_list
-      (Partial_Annotated_Clausal_Logic.equal_marked_lit Arith.equal_int
+      (Partial_Annotated_Clausal_Logic.equal_ann_literal Arith.equal_int
         Product_Type.equal_unit Product_Type.equal_unit))
     (List.equal_list
       (List.equal_list (Clausal_Logic.equal_literal Arith.equal_int)))
